Assignment12 Done.

sf/Assignment12_05.v
@@ -13,31 +13,86 @@ Require Export Assignment12_04.
 *)
 
 Definition halve : tm :=
-  FILL_IN_HERE.
+    tfix (tabs Halve (TArrow TNat TNat) 
+        (tabs X TNat (tif0 (tvar X) (tnat 0) 
+            (tif0 (tpred (tvar X)) (tnat 0) (tsucc (tapp (tvar Halve) (tpred (tpred (tvar X))))))))).
 
 Example halve_type: empty |- halve \in TArrow TNat TNat.
 Proof.
+  unfold halve; eauto 10.
   (* unfold halve; eauto 10. *)
-  exact FILL_IN_HERE.
 Qed.
 
 Example halve_10: tapp halve (tnat 10) ==>* tnat 5.
 Proof.
+  unfold halve; normalize.
   (* unfold halve; normalize. *)
-  exact FILL_IN_HERE.
 Qed.
 
 Example halve_11: tapp halve (tnat 11) ==>* tnat 5.
 Proof.
+  unfold halve; normalize.
   (* unfold halve; normalize. *)
-  exact FILL_IN_HERE.
+Qed.
+
+Lemma lem_f1 : forall t1 t2,
+    t1 ==>* t2 -> tsucc t1 ==>* tsucc t2.
+Proof.
+    intros.
+    induction H.
+    constructor.
+    eapply multi_step.
+    constructor.
+    apply H.
+    apply IHmulti.
 Qed.
 
 
 Theorem halve_correct: forall n,
    tapp halve (tnat (n+n)) ==>* tnat n.
 Proof.
-  exact FILL_IN_HERE.
+    intros.
+    induction n.
+    simpl.
+    unfold halve; normalize.
+    unfold halve.
+    eapply multi_step.
+    eapply ST_AppFix.
+    eauto.
+    eauto.
+    eapply multi_step.
+    eapply ST_App1.
+    eauto.
+    simpl.
+    eapply multi_step.
+    eapply ST_AppAbs.
+    eauto.
+    simpl.
+    eapply multi_step.
+    eapply ST_If0Nonzero.
+    eapply multi_step.
+    eapply ST_If01.
+    eapply ST_PredNat.
+    simpl.
+    eapply multi_step.
+    rewrite <- plus_n_Sm.
+    eapply ST_If0Nonzero.
+    eapply multi_step.
+    eapply ST_Succ1.
+    eapply ST_App2.
+    eauto.
+    eauto.
+    eapply multi_step.
+    eapply ST_Succ1.
+    eapply ST_App2.
+    eauto.
+    eauto.
+    apply lem_f1 in IHn.
+    apply multi_trans with (y := tsucc (tnat n)).
+    apply IHn.
+    eapply multi_step.
+    eapply ST_SuccNat.
+    constructor.
 Qed.
 
 (*-- Check --*)
