sf/Assignment12_06.v
@@ -2,10 +2,159 @@ Require Export Assignment12_05.
 
 (* problem #06: 10 points *)
 
+Notation Loop_step1 := (tapp tloop (tnat 0)).
+Notation Loop_step2 := (tapp
+  (tapp
+     (tabs Loop (TArrow TNat TNat) (tabs X TNat (tapp (tvar Loop) (tvar X))))
+     (tfix
+        (tabs Loop (TArrow TNat TNat)
+           (tabs X TNat (tapp (tvar Loop) (tvar X)))))) (tnat 0)).
+Notation Loop_step3 := (tapp
+  ([Loop
+   := tfix
+        (tabs Loop (TArrow TNat TNat)
+           (tabs X TNat (tapp (tvar Loop) (tvar X))))]
+   tabs X TNat (tapp (tvar Loop) (tvar X))) (tnat 0)).
+
+Inductive multi_n_step : tm -> nat -> tm -> Prop :=
+    | zero_step : forall t, multi_n_step t 0 t
+    | succ_step : forall n t0 t1 t2, 
+        t0 ==> t1 -> multi_n_step t1 n t2 -> multi_n_step t0 (S n) t2.
+
+Lemma multi_n_step_exists : forall t1 t2,
+    t1 ==>* t2 -> exists n, (multi_n_step t1 n t2).
+Proof.
+    intros.
+    induction H.
+    exists 0.
+    constructor.
+    inversion IHmulti.
+    exists (S x0).
+    apply succ_step with (t1 := y).
+    apply H.
+    apply H1.
+Qed.
+    
+
+Lemma loop_three : forall x n,
+    multi_n_step Loop_step1 n x \/ multi_n_step Loop_step2 n x \/ multi_n_step Loop_step3 n x
+        -> x = Loop_step1 \/ x = Loop_step2 \/ x = Loop_step3.
+Proof.
+    intros.
+    generalize dependent x.
+    induction n.
+    intros.
+    inversion H.
+    inversion H0.
+    left; auto.
+    inversion H0.
+    inversion H1.
+    subst.
+    auto.
+    inversion H1.
+    subst.
+    auto.
+    intros.
+    inversion H.
+    inversion H0.
+    subst.
+    assert (t1 = Loop_step2).
+        inversion H2.
+        subst.
+        inversion H6.
+        subst.
+        inversion H3.
+        subst.
+        inversion H5.
+        subst.
+        inversion H7.
+        subst.
+        auto.
+    rewrite H1 in H4.
+    assert (multi_n_step Loop_step1 n x \/ multi_n_step Loop_step2 n x \/ multi_n_step Loop_step3 n x).
+        auto.
+    apply IHn in H3.
+    apply H3.
+    inversion H0.
+    inversion H1.
+    subst.
+    assert (t1 = Loop_step3).
+        inversion H3.
+        subst.
+        inversion H7.
+        subst.
+        inversion H10.
+        subst.
+        auto.
+        inversion H8.
+        subst.
+        inversion H9.
+        subst.
+        inversion H4.
+        subst.
+        inversion H8.
+    rewrite H2 in H5.
+    assert (multi_n_step Loop_step1 n x \/ multi_n_step Loop_step2 n x \/ multi_n_step Loop_step3 n x).
+        auto.
+    apply IHn in H4.
+    apply H4.
+    inversion H1.
+    subst.
+    assert (t1 = Loop_step1).
+        inversion H3.
+        subst.
+        auto.
+        subst.
+        inversion H7.
+        subst.
+        inversion H8.
+    rewrite H2 in H5.
+    assert (multi_n_step Loop_step1 n x \/ multi_n_step Loop_step2 n x \/ multi_n_step Loop_step3 n x).
+        auto.
+    apply IHn in H4.
+    auto.
+Qed.
+
+Lemma loop_one : forall x,
+    Loop_step1 ==>* x -> x = Loop_step1 \/ x = Loop_step2 \/ x = Loop_step3.
+Proof.
+    intros.
+    apply multi_n_step_exists in H.
+    inversion H.
+    inversion H0.
+    subst.
+    left; auto.
+    subst.
+    apply loop_three with (n := (S n)).
+    left; auto.
+Qed.
+
 Theorem tloop_diverges:
   ~ exists t, tapp tloop (tnat 0) ==>* t /\ normal_form step t.
 Proof.
-  exact FILL_IN_HERE.
+    unfold not.
+    intros.
+    inversion H.
+    unfold normal_form in H0.
+    inversion H0.
+    unfold not in H2.
+    apply H2.
+    apply loop_one in H1.
+    inversion H1.
+    exists Loop_step2.
+    rewrite H3.
+    eapply ST_AppFix.
+    constructor.
+    constructor.
+    inversion H3.
+    exists Loop_step3.
+    rewrite H4.
+    eapply ST_App1.
+    auto.
+    rewrite H4.
+    exists Loop_step1.
+    apply ST_AppAbs.
+    constructor.
 Qed.
 
 (*-- Check --*)
