sf/Assignment12_04.v
@@ -7,9 +7,28 @@ Corollary soundness : forall t t' T,
   t ==>* t' ->
   ~(stuck t').
 Proof.
-  exact FILL_IN_HERE.
+    intros.
+    unfold stuck.
+    unfold not.
+    intros.
+    unfold normal_form in H1.
+    unfold not in H1.
+    inversion H1.
+    apply H3.
+    induction H0.
+    apply progress in H.
+    inversion H.
+    apply H0.
+    apply H2 in H0.
+    inversion H0.
+    apply IHmulti.
+    apply preservation with (t' := y) in H.
+    apply H.
+    apply H0.
+    apply H1.
+    apply H2.
+    apply H3.
 Qed.
-
 (*-- Check --*)
 Check soundness : forall t t' T,
   empty |- t \in T -> 
